Fix error propagation logic in promise-first mode (#54)
Also make GenPromising contain more logic meaning less duplication in both promise-first and regular exploration.

ArchSem/GenPromising.v
@@ -136,69 +136,77 @@ Module GenPromising (IWA : InterfaceWithArch) (TM : TermModelsT IWA).
   Import IWA.Interface.
   Import TM.
 
-  Structure PromisingModel := {
+  (* Namespace *)
+  Module Promising.
+
+  (** This structure defines a promising model that can share common
+      infrastructure define in this file. This structure allows to define 4
+      models:
+      - The non-certified non-executable version where any promises can be made
+        as long as they are all fulfilled by the end
+      - The certified non-executable version where promises can only be made if
+        there is a sequential trace that lead to that promise being fulfilled.
+      - The direct executable model which explores all interleaving of promising
+        and instruction steps
+      - The promise-free executable model which does a smarter search based on
+        some commutation properties of steps, namely that instruction step of
+        different thread commute and that a promise step after an instruction
+        step can always be commuted to be before.
+
+      The first one is there for theoretical reason, but it probably can return
+      UB on any input, but any non-error behavior it exhibits should also be in
+      the certified version, so it can be useful for sanity checking.
+
+      Theoretically the last 3 models are equivalent (up to fuel for the
+      executable ones).
+
+      TODO: Figure out generic properties to relate those 4 models.
+   *)
+  Structure Model := {
+      (** The thread state of the model *)
       tState : Type;
+      (** Initialize the model thread state from architectural state *)
       tState_init : (* tid *) nat → memoryMap → registerMap → tState;
+      (** Get a register map out of a thread state to test the termination
+          condition and compute a final state *)
       tState_regs : tState → registerMap;
+      (** Check if a thread state has no pending promises, which means that it
+          can be explained with the current memory state *)
       tState_nopromises : tState → bool;
       (** Intra instruction state, reset after each instruction *)
       iis : Type;
       iis_init : iis;
+      (** The type of memory event, any communication between threads must go here *)
       mEvent : Type;
+      mEvent_eq_dec : EqDecision mEvent;
+      (** Give the tid that initiated that event *)
+      mEvent_tid : mEvent → nat;
+      (** The address space this model is built against, we expect non-secure
+          for Arm here *)
       address_space : addr_space;
-      handler : (* tid *) nat → memoryMap →
-                fHandler outcome
-                  (Exec.t (PPState.t tState mEvent iis) string);
-      allowed_promises : (* tid *) nat → memoryMap → tState →
-                         PromMemory.t mEvent → propset mEvent;
-      (** Update the thread state after emission of a promise.
-          The new promise has been added to the memory when calling that function.
-          I'm not considering that emit_promise can fail or have a
-          non-deterministic behaviour *)
+      (** The handler for instruction effects, applies the effect of a single
+          outcome to the thread state. If the outcome need one or more event to
+          be added to memory,it adds them and return the view of those events in
+          the option, otherwise it returns [None] *)
+      handle_outcome : (* tid *) nat → (* initial memory *) memoryMap →
+                  ∀ out : outcome,
+                  Exec.t (PPState.t tState mEvent iis) string
+                         (eff_ret out * option nat);
+      (** Update the thread state after emission of a promise. The new promise
+          has already been added to the memory when calling that function. I'm
+          not considering that emit_promise can fail or have a non-deterministic
+          behaviour. TODO: Add support for failure *)
       emit_promise : (* tid *) nat → memoryMap → PromMemory.t mEvent →
                      mEvent → tState → tState;
+      (** Hook for extra UB checks to be done before returning a final state,
+          e.g. BBM checks. Any returned string is an error, [[]] is success. *)
+      check_valid_end : (* tid *) nat → memoryMap → tState →
+                             PromMemory.t mEvent → list string;
+      (** Computes the final memory after a certain promising history *)
       memory_snapshot : memoryMap → PromMemory.t mEvent → memoryMap;
     }.
-  Arguments PromisingModel : clear implicits.
-
-  (** This is a basic way of making a promising model executable, so I'll make
-      it generic *)
-  Structure BasicExecutablePM := {
-      pModel :> PromisingModel;
-
-      enumerate_promises_and_terminal_states :
-        (* fuel *) nat → (* tid *) nat →
-        (* termination condition *) (registerMap → bool) →
-        memoryMap → pModel.(tState) → PromMemory.t pModel.(mEvent) →
-        result string (list pModel.(mEvent) * list pModel.(tState));
-
-      promise_select_sound :
-        ∀ fuel tid term initMem ts mem promises tstates,
-          Ok (promises, tstates) =
-            enumerate_promises_and_terminal_states fuel tid term initMem ts mem →
-          ∀ ev ∈ promises, ev ∈ pModel.(allowed_promises) tid initMem ts mem;
-
-      promise_select_complete :
-        ∀ fuel tid term initMem ts mem promises tstates,
-          Ok (promises, tstates) =
-            enumerate_promises_and_terminal_states fuel tid term initMem ts mem →
-          ∀ ev ∈ pModel.(allowed_promises) tid initMem ts mem, ev ∈ promises;
-
-      terminal_state_no_outstanding_promise :
-        ∀ fuel tid term initMem ts mem promises tstates,
-          Ok (promises, tstates) =
-            enumerate_promises_and_terminal_states fuel tid term initMem ts mem →
-          ∀ tts ∈ tstates, pModel.(tState_nopromises) tts;
-
-      terminal_state_is_terminated :
-        ∀ fuel tid term initMem ts mem promises tstates,
-          Ok (promises, tstates) =
-            enumerate_promises_and_terminal_states fuel tid term initMem ts mem →
-          ∀ tts ∈ tstates, term (pModel.(tState_regs) tts);
-
-      (* TODO: add terminal_state_is_reachable *)
-    }.
-  Arguments BasicExecutablePM : clear implicits.
+  #[global] Arguments Model : clear implicits.
+  End Promising.
 
   Module PState. (* namespace *)
     Section PS.
@@ -221,8 +229,9 @@ Module GenPromising (IWA : InterfaceWithArch) (TM : TermModelsT IWA).
     Arguments t : clear implicits.
 
     Section PSProm.
+      Import Promising.
       Context (isem : iMon ()).
-      Context (prom : PromisingModel).
+      Context (prom : Model).
       Context {n : nat}.
       Local Notation tState := prom.(tState).
       Local Notation mEvent := prom.(mEvent).
@@ -243,6 +252,14 @@ Module GenPromising (IWA : InterfaceWithArch) (TM : TermModelsT IWA).
       (** Check if all threads have no outstanding promises *)
       Definition nopromises (ps : t) := fforallb (nopromises_tid ps).
 
+      (** Check if a thread state can be at a valid end *)
+      Definition check_valid_end_tid (ps : t) (tid : fin n) :=
+        prom.(check_valid_end) tid ps.(initmem) (tstate tid ps) ps.(events).
+
+      (** Check if all thread states can be at a valid end *)
+      Definition check_valid_end (ps : t) :=
+        List.concat (map (check_valid_end_tid ps) (enum (fin n))).
+
       Definition PState_PPState tid (pst : t) :
           PPState.t tState mEvent prom.(iis) :=
         PPState.Make (tstate tid pst) pst.(events) prom.(iis_init).
@@ -254,34 +271,44 @@ Module GenPromising (IWA : InterfaceWithArch) (TM : TermModelsT IWA).
           |> setv (tstate tid) ppst.(PPState.state)
           |> setv events ppst.(PPState.mem).
 
-      (** Run on instruction in specific thread by tid *)
+      (** Run on instruction in specific thread by tid, allowing new promises *)
       Definition run_tid (tid : fin n) : Exec.t t string () :=
         st ← mGet;
-        let handler := prom.(handler) tid (st.(initmem)) in
+        let handler out := prom.(handle_outcome) tid (st.(initmem)) out |$> fst in
         Exec.liftSt (PState_PPState tid) (cinterp handler isem).
 
+      Definition seq_step (tid : fin n) : relation t :=
+        λ st1 st2, st2 ∈ Exec.success_state_list $ run_tid tid st1.
+
       (** Compute the set of allowed promises by a thread indexed by tid *)
-      Definition allowed_promises_tid (st : t) (tid : fin n) :=
-        prom.(allowed_promises) tid st.(initmem) (tstate tid st) st.(events).
+      Definition allowed_promises_tid (certified : bool) (st : t) (tid : fin n)
+        (ev : mEvent) :
+          Prop :=
+        if certified then
+          let st_plus := set PState.events (ev ::.) st in
+          ∃ st', rtc (seq_step tid) st_plus st' ∧
+                   nopromises_tid st tid
+        else prom.(mEvent_tid) ev = tid.
 
       (** Emit a promise from a thread by tid *)
-      Definition promise_tid (st : t) (tid : fin n) (event : mEvent) :=
+      Definition promise_tid (tid : fin n) (event : mEvent) (st : t) :=
         let st := set events (event ::.) st in
         set (tstate tid)
           (prom.(emit_promise) tid st.(initmem) st.(events) event)
           st.
 
       (** The inductive stepping relation of the promising model *)
-      Inductive step (ps : t) : (t) -> Prop :=
+      Inductive step (certified : bool) (ps : t) : (t) -> Prop :=
       | SRun (tid : fin n) (ps' : t) :
-        (ps', ()) ∈ (run_tid tid ps) → step ps ps'
+        (ps', ()) ∈ (run_tid tid ps) → step certified ps ps'
       | SPromise (tid : fin n) (event : mEvent) :
-        event ∈ allowed_promises_tid ps tid → step ps (promise_tid ps tid event).
+        allowed_promises_tid certified ps tid event →
+        step certified ps (promise_tid tid event ps).
 
-      Lemma step_promise (ps ps' : t) (tid : fin n) (event : mEvent) :
-        event ∈ allowed_promises_tid ps tid →
-        ps' = promise_tid ps tid event →
-        step ps ps'.
+      Lemma step_promise certified (ps ps' : t) (tid : fin n) (event : mEvent) :
+        allowed_promises_tid certified ps tid event →
+        ps' = promise_tid tid event ps →
+        step certified ps ps'.
       Proof using. sauto l:on. Qed.
 
       (** Create an initial promising state from a generic machine state *)
@@ -305,34 +332,45 @@ Module GenPromising (IWA : InterfaceWithArch) (TM : TermModelsT IWA).
   End PState.
 
   (** Create a non-computational model from an ISA model and promising model *)
-  Definition Promising_to_Modelnc (isem : iMon ()) (prom : PromisingModel)
-    : archModel.nc ∅ :=
+  Definition Promising_to_Modelnc (certified : bool) (prom : Promising.Model)
+       (isem : iMon ()) : archModel.nc ∅ :=
     λ n term (initMs : archState n),
       {[ mr : archModel.res ∅ n term |
          let initPs := PState.from_archState prom initMs in
          match mr with
          | archModel.Res.FinalState fs _ =>
-             ∃ finPs, rtc (PState.step isem prom) initPs finPs ∧
+             ∃ finPs, rtc (PState.step isem prom certified) initPs finPs ∧
                         PState.to_archState prom finPs = fs ∧
-                        PState.nopromises prom finPs
+                        PState.nopromises prom finPs ∧
+                        PState.check_valid_end prom finPs = []
          | archModel.Res.Error s =>
-             ∃ finPs tid, rtc (PState.step isem prom) initPs finPs ∧
-                            Error s ∈ PState.run_tid isem prom tid finPs
+             ∃ finPs,
+              rtc (PState.step isem prom certified) initPs finPs ∧
+                ((∃ tid, Error s ∈ PState.run_tid isem prom tid finPs)
+                  ∨
+                 (PState.terminated prom term finPs ∧
+                  PState.nopromises prom finPs ∧
+                  s ∈ PState.check_valid_end prom finPs))
          | _ => False
          end]}.
 
   (** Computational promising state. Right now it the same type as PState.t but
       with more methods *)
   Module CPState.
+    Import Promising.
     Include PState.
     Section CPS.
     Context (isem : iMon ()).
-    Context (prom : BasicExecutablePM).
+    Context (prom : Model).
     Context {n : nat}.
     Context (term : terminationCondition n).
     Local Notation tState := (tState prom).
     Local Notation mEvent := (mEvent prom).
+    Local Notation iis := (iis prom).
     Local Notation t := (t tState mEvent n).
+
+    Let mEvent_eq_dec := prom.(mEvent_eq_dec).
+    Local Existing Instance mEvent_eq_dec.
 
     (** The type of final promising state return by run *)
     Definition final := { x : t | terminated prom term x }.
@@ -346,22 +384,92 @@ Module GenPromising (IWA : InterfaceWithArch) (TM : TermModelsT IWA).
     Solve All Obligations with
       hauto unfold:terminated unfold:archState.is_terminated l:on db:vec, brefl.
 
+
+    Section EnumerateResult.
+      Context (tid : fin n) (initmem : memoryMap).
+
+      Definition run_outcome_with_promise (base : nat) (out : outcome) :
+          Exec.t (list mEvent * PPState.t tState mEvent iis) string (eff_ret out) :=
+        '(res, vpre_opt) ← Exec.liftSt snd $ prom.(handle_outcome) tid initmem out;
+        if vpre_opt is Some vpre then
+          if decide (vpre ≤ base)%nat then
+            mem ← mget (PPState.mem ∘ snd);
+            (* Take all promises after base (made by that outcome) and add them
+               to the list of possible new promises *)
+            mset fst (take (length mem - base) mem ++.);;
+            mret res
+          else mret res
+        else
+          mret res.
+
+      Fixpoint run_to_termination (fuel : nat) (base : nat) :
+          Exec.t (list mEvent * PPState.t tState mEvent iis) string bool :=
+        match fuel with
+        | 0%nat =>
+            ts ← mget (PPState.state ∘ snd);
+            mret (term tid (prom.(tState_regs) ts))
+        | S fuel =>
+            let handler := run_outcome_with_promise base in
+            cinterp handler isem;;
+            ts ← mget (PPState.state ∘ snd);
+            if term tid (prom.(tState_regs) ts) then
+              mret true
+            else
+              msetv (PPState.iis ∘ snd) prom.(iis_init);;
+              run_to_termination fuel base
+        end.
+
+      Record EnumerationResult :=
+        {
+          promises : list mEvent;
+          final_states : list tState;
+          errors : list string;
+          out_of_fuel : bool
+        }.
+
+      Definition enumerate_results (fuel : nat) (ts : tState)
+          (mem : PromMemory.t mEvent) : EnumerationResult :=
+        let base := List.length mem in
+        let res :=
+          run_to_termination fuel base
+            ([], PPState.Make ts mem prom.(iis_init))
+        in
+        let success_states := Exec.success_state_list res in
+        let out_of_fuel := bool_decide (∃ r ∈ (Exec.results res).*2, ¬ (r : bool)) in
+        (* let out_of_fuel := true in *)
+        let promises := List.concat (success_states.*1) |> remove_dups in
+        let tstates :=
+          success_states
+          |> omap (λ '(new_proms, st),
+                 if is_emptyb new_proms then Some (PPState.state st)
+                 else None) in
+        let errors :=
+          res |> Exec.errors |>
+            omap (λ '((new_proms, _), err_msg),
+                if is_emptyb new_proms then Some err_msg
+                else None) in
+        {|promises:=promises;
+          final_states:=tstates;
+          errors:=errors;
+          out_of_fuel:=out_of_fuel|}.
+    End EnumerateResult.
+
     (** Get a list of possible promises for a thread by tid *)
     Definition promise_select_tid (fuel : nat) (st : t)
         (tid : fin n) : Exec.res string mEvent :=
-      '(promises, _) ← mlift $ prom.(enumerate_promises_and_terminal_states)
-                        fuel tid (term tid) (initmem st) (tstate tid st) (events st);
-      mchoosel promises.
+      let (promises, _, _, out_of_fuel) :=
+        enumerate_results tid (initmem st) fuel (tstate tid st) (events st)
+      in
+      if out_of_fuel then
+        b ← mchoosef;
+        if (b : bool) then mthrow "out of fuel" else mchoosel promises
+      else mchoosel promises.
 
     (** Take any promising step for that tid and promise it *)
-    Definition cpromise_tid (fuel : nat) (tid : fin n)
-      : Exec.t t string () :=
-    λ st,
-      let res_st :=
-        ev ← promise_select_tid fuel st tid;
-        mret $ promise_tid prom st tid ev
-      in
-        Exec.make ((.,()) <$> res_st.(Exec.results)) ((st,.) <$> res_st.(Exec.errors)).
+    Definition cpromise_tid (fuel : nat) (tid : fin n) : Exec.t t string () :=
+      st ← mGet;
+      ev ← mlift (promise_select_tid fuel st tid);
+      mSetv (promise_tid prom tid ev st).
 
     (** Run any possible step, this is the most exhaustive and expensive kind of
         search but it is obviously correct. If a thread has reached termination
@@ -392,42 +500,52 @@ Module GenPromising (IWA : InterfaceWithArch) (TM : TermModelsT IWA).
     Fixpoint run_promise_first (fuel : nat) : Exec.t t string final :=
       if fuel is S fuel then
         st ← mGet;
-        (* Find out next possible promises or terminating states at the current thread *)
-        executions ←
-          vmapM (λ '(tid, ts),
-            '(promises_per_tid, tstates_per_tid) ←
-              mlift $ prom.(enumerate_promises_and_terminal_states)
-                        fuel (fin_to_nat tid) (term tid) (initmem st) ts (events st);
-            mret (map (.,tid) promises_per_tid, tstates_per_tid)
-          ) (venumerate (tstates st));
-
-        promise ← mchoosel (enum bool);
-        if (promise : bool) then
-          (* Non-deterministically choose the next promise and the tid for pruning *)
-          let promises_all := List.concat (vmap fst executions) in
-          '(next_ev, tid) ← mchoosel promises_all;
-          mSet (λ st, promise_tid prom st tid next_ev);;
+        (* Find out next possible promises or terminating states for each thread *)
+        let execution_results :=
+          vmap (λ '(tid, ts),
+              enumerate_results tid (initmem st) fuel ts (events st)
+            ) (venumerate (tstates st)) in
+        opt ← mchoosel (seq 0 4);
+        match opt : nat with
+        | 0 =>
+          '(tid : fin n) ← mchoosef;
+          next_ev ← mchoosel (execution_results !!! tid).(promises);
+          mSet (promise_tid prom tid next_ev);;
           run_promise_first fuel
-        else
+        | 1 =>
           (* Compute cartesian products of the possible thread states *)
-          let tstates_all := cprodn (vmap snd executions) in
-          let new_finals :=
-            omap (λ tstates,
-              let st := Make tstates st.(PState.initmem) st.(PState.events) in
-              if decide $ terminated prom term st is left pt
-              then Some (make_final st pt)
-              else None
-            ) tstates_all in
-          mchoosel new_finals
+          tstates ← mchoosel $ cprodn (vmap final_states execution_results);
+          (* Lift them into full promising state *)
+          let st := Make tstates st.(initmem) st.(events) in
+          (* Discard the one with pending promises in any thread *)
+          guard_discard $ nopromises prom st;;
+          (* Discard the non-terminated ones *)
+          term_proof ← guard_discard $ terminated prom term st;
+          (* Check for final errors (e.g. BBM checks) *)
+          let errs := check_valid_end prom st in
+          if errs is [] then
+            mret (make_final st term_proof)
+          else
+            err ← mchoosel errs;
+            mthrow err
+        | 2 =>
+          let errs := List.concat (vmap errors execution_results) in
+          err ← mchoosel errs;
+          mthrow err
+        | _ =>
+          if bool_decide (∃ x ∈ map out_of_fuel execution_results, (x : bool)) then
+            mthrow "Promise first: out of fuel in enumeration"
+          else mdiscard
+        end
       else
-        mthrow "Could not finish running within the size of the fuel".
+        mthrow "Promise first: out of fuel in main loop".
 
     End CPS.
     Arguments to_final_archState {_ _ _}.
   End CPState.
 
   (** Create computational models from an ISA model and promising model *)
-  Definition Promising_to_Modelc (isem : iMon ()) (prom : BasicExecutablePM)
+  Definition Promising_to_Modelc (prom : Promising.Model) (isem : iMon ())
       (fuel : nat) : archModel.c ∅ :=
     λ n term (initMs : archState n),
       PState.from_archState prom initMs |>
@@ -435,13 +553,13 @@ Module GenPromising (IWA : InterfaceWithArch) (TM : TermModelsT IWA).
         $ CPState.to_final_archState
         <$> CPState.run isem prom term fuel.
 
-  Definition Promising_to_Modelc_pf (isem : iMon ()) (prom : BasicExecutablePM)
+  Definition Promising_to_Modelc_pf (prom : Promising.Model) (isem : iMon ())
       (fuel : nat) : archModel.c ∅ :=
     λ n term (initMs : archState n),
       PState.from_archState prom initMs |>
       archModel.Res.from_exec
         $ CPState.to_final_archState
-        <$> CPState.run_promise_first prom term fuel.
+        <$> CPState.run_promise_first isem prom term fuel.
 
 End GenPromising.
 
